\begin{gather*}
d(tr(AX^{-T}BXC)) = 
tr(d(AX^{-T}BXC)) = \\
tr\left\lbrace (d(AX^{-T}B))XC + AX^{-T}Bd(XC) \right\rbrace  = \\
tr\left\lbrace A(dX^{-1})^TBXC + AX^{-T}B(dX)C \right\rbrace  = \\
tr\left\lbrace -AX^{-T}(dX)^TX^{-T}BXC + AX^{-T}B(dX)C \right\rbrace  = \\
-tr\left\lbrace X^{-T}BXCAX^{-T}(dX)^T \right\rbrace + \
tr\left\lbrace CAX^{-T}BdX           \right\rbrace  = \\
-tr\left\lbrace (X^{-T}BXCAX^{-T}(dX)^T)^T \right\rbrace + \
tr\left\lbrace CAX^{-T}BdX           \right\rbrace  = \\
-tr\left\lbrace (dX)X^{-1}A^TC^TX^TB^TX^{-1} \right\rbrace + \
tr\left\lbrace CAX^{-T}BdX           \right\rbrace  = \\
-tr\left\lbrace X^{-1}A^TC^TX^TB^TX^{-1}dX \right\rbrace + \
tr\left\lbrace CAX^{-T}BdX           \right\rbrace  = \\
tr\left\lbrace -X^{-1}A^TC^TX^TB^TX^{-1}dX + \
CAX^{-T}BdX           \right\rbrace  = \\
tr\left\lbrace \right(-X^{-1}A^TC^TX^TB^TX^{-1} + \
CAX^{-T}B \left) dX           \right\rbrace  = \\
\left< I_n, \right(-X^{-1}A^TC^TX^TB^TX^{-1} + \
CAX^{-T}B \left) dX \right> = \\
\left< \right(-X^{-1}A^TC^TX^TB^TX^{-1} + \
CAX^{-T}B \left)^T, dX \right> = \\
\left< B^TX^{-1}A^TC^T - X^{-T}BXCAX^{-T} , dX \right> \\
\rightarrow \quad \dfrac{\partial}{\partial X} tr(AX^{-T}BXC) = \
B^TX^{-1}A^TC^T - X^{-T}BXCAX^{-T}
\end{gather*}